ocaml/main.ml
@@ -4,6 +4,8 @@ open Openflow1_0
 open Platform 
 open Unix
 
+module M = MonadicController
+
 module ServerFd : Platform.FD = struct
   let fd = socket PF_INET SOCK_STREAM 0
     
