ocaml/monadicController.ml
@@ -1,0 +1,64 @@
+open MessagesDef
+open ControllerInterface
+
+module type STATE = sig
+  type state
+end
+
+module Make 
+  (Platform : Platform.PLATFORM) 
+  (State : STATE) : CONTROLLER_MONAD = struct
+
+  type state = State.state
+      
+  type 'x m = state -> 'x * state
+
+  let bind (m : 'a m) (k : 'a -> 'b m) : 'b m = fun s ->
+    let (a, s') = m s in k a s'
+
+  let ret (a : 'a) : 'a m = fun (s : state) -> (a,s)
+
+  let get : state m = fun s -> (s,s)
+
+  let put (s : state) : unit m = fun _ -> ((), s)
+
+  let rec forever (m : unit m) = bind m (fun _ -> forever m)
+
+  let events : event Event.channel = Event.new_channel ()
+
+  let send (sw_id : switchId) (xid : xid) (msg : message) = fun (s : state) ->
+    begin
+      try 
+        Platform.send_to_switch sw_id xid msg        
+      with Platform.SwitchDisconnected sw_id' ->
+        Event.sync (Event.send events (SwitchDisconnected sw_id'))
+    end;
+    ((), s)
+
+  let recv : event m = fun (s : state) ->
+    (Event.sync (Event.receive events), s)
+
+  let recv_from_switch_thread sw_id = 
+    try
+      let rec loop () = 
+        let (xid, msg) = Platform.recv_from_switch sw_id in
+        Event.sync (Event.send events (SwitchMessage (sw_id, xid, msg)));
+        loop () in
+      loop ()
+    with Platform.SwitchDisconnected sw_id' ->
+      Event.sync (Event.send events (SwitchDisconnected sw_id'))
+
+  let rec accept_switch_thread () = 
+    let feats = Platform.accept_switch () in
+    Event.sync (Event.send events (SwitchConnected feats.switch_id));
+    let _ = Thread.create recv_from_switch_thread feats.switch_id in
+    accept_switch_thread ()
+
+
+  let run (init : state) (action : 'a m) : 'a = 
+    (** TODO(arjun): kill threads etc. *)
+    let _ = Thread.create accept_switch_thread () in
+    let (result, _) = action init in
+    result
+
+  end
