coq/Classifier/Defs.v
@@ -58,4 +58,3 @@ Fixpoint elim_shadowed_helper {A : Type} (prefix : Classifier A)
 
 Definition elim_shadowed {A : Type} (cf : Classifier A) :=
   elim_shadowed_helper nil cf.
-
