coq/Extraction/Extract.v
@@ -3,7 +3,8 @@ Require Import NArith.BinNat.
 
 Require Import OpenFlow.MessagesDef.
 Require Import Extraction.OCaml.
+Require Import NetCore.NetCoreController.
 
 Cd "../../ocaml/extracted". 
-Recursive Extraction Library MessagesDef.
 Recursive Extraction Library OCaml.
+Recursive Extraction Library NetCoreController.
