coq/NetCore/NetCoreController.v
@@ -1,0 +1,169 @@
+Set Implicit Arguments.
+
+Require Import Common.Types.
+Require Import Common.Monad.
+Require Import Word.WordInterface.
+Require Import Network.Packet.
+Require Import OpenFlow.MessagesDef.
+Require Import Pattern.Defs.
+Require Import Classifier.Defs.
+Require Import NetCore.NetCore.
+Require Import OpenFlow.ControllerInterface.
+
+Local Open Scope list_scope.
+
+Section Prioritize.
+
+  (** TODO(arjun): deal with priority overflowing 16 bits *)
+  Fixpoint prio_rec {A : Type} (prio : Word16.t) (lst : Classifier A) :=
+    match lst with
+      | nil => nil
+      | (pat, act) :: rest => 
+        (prio, pat, act) :: (prio_rec (Word16.pred prio) rest)
+    end.
+
+  Definition prioritize {A : Type} (lst : Classifier A) :=
+    prio_rec Word16.max_value lst.
+
+End Prioritize.
+
+Section ToFlowMod.
+
+  Definition translate_action (act : Action) :=
+    match act with
+      | Forward pp => Output pp
+      | ActGetPkt x => Output (Controller Word16.max_value)
+    end.
+
+  Definition to_flow_mod prio (pat : Pattern) (act : list Action)
+             (isfls : Pattern.is_empty pat = false) :=
+    FlowMod AddFlow
+            (Pattern.to_match pat isfls)
+            prio
+            (List.map translate_action act)
+            Word32.zero
+            Permanent
+            Permanent
+            false
+            None
+            None
+            true.
+
+  Definition flow_mods_of_classifier lst :=
+    List.fold_right
+      (fun (ppa : priority * Pattern * list Action)
+           (lst : list flowMod) => 
+         match ppa with
+           | (prio,pat,act) => 
+             (match (Pattern.is_empty pat) as b
+                    return (Pattern.is_empty pat = b -> list flowMod) with
+                | true => fun _ => lst
+                | false => fun H => (to_flow_mod prio pat act H) :: lst
+              end) eq_refl
+         end)
+      nil
+      (prioritize lst).
+
+  Lemma Pattern_all_not_empty : Pattern.is_empty Pattern.all = false.
+  Proof.
+    unfold Pattern.is_empty.
+    reflexivity.
+  Qed.
+
+  Definition delete_all_flows := 
+    FlowMod DeleteFlow
+            (* This should make reasoning easier, since we have so many
+               theorems about patterns. *)
+            (Pattern.to_match Pattern.all Pattern_all_not_empty)
+            Word16.zero
+            nil
+            Word32.zero
+            Permanent
+            Permanent
+            false
+            None
+            None
+            true.
+
+
+End ToFlowMod.
+
+
+Module Type NETCORE_MONAD <: CONTROLLER_MONAD.
+
+  Include MONAD.
+
+  Record ncstate := State {
+    policy : Pol;
+    switches : list switchId
+  }.
+
+  Definition state := ncstate.
+
+  Parameter get : m state.
+  Parameter put : state -> m unit.
+  Parameter send : switchId -> xid -> message -> m unit.
+  Parameter recv : m event.
+
+  (** Must be defined in OCaml *)
+  Parameter forever : m unit -> m unit.
+
+End NETCORE_MONAD.
+
+Module Make (Import Monad : NETCORE_MONAD).
+
+  Local Notation "x <- M ; K" := (bind M (fun x => K)).
+  Check compile_pol.
+
+  Fixpoint sequence (lst : list (m unit)) : m unit := 
+    match lst with
+      | nil => ret tt
+      | cmd :: lst' =>
+        bind cmd (fun _ => sequence lst')
+    end.
+  
+  Definition config_commands (pol: Pol) (swId : switchId) :=
+    sequence
+      (List.map
+         (fun fm => send swId Word32.zero (FlowModMsg fm))
+         (delete_all_flows 
+            :: (flow_mods_of_classifier (compile_opt pol swId)))).
+
+  Definition set_policy (pol : Pol) := 
+    st <- get;
+    let switch_list := switches st in
+    _ <- put (State pol switch_list);
+    _ <- sequence (List.map (config_commands pol) switch_list);
+    ret tt.
+
+  Definition handle_switch_disconnected (swId : switchId) :=
+    st <- get;
+    let switch_list := 
+        List.filter 
+          (fun swId' => match Word64.eq_dec swId swId' with
+                          | left _ => false
+                          | right  _ => true
+                        end)
+          (switches st) in
+    _ <- put (State (policy st) switch_list);
+    ret tt.
+
+  (** TODO(arjun): I'm assuming we don't disconnected and connected are
+      interleaved. OCaml should provide that guarantee. *)
+  Definition handle_switch_connected (swId : switchId) :=
+    st <- get;
+    _ <- put (State (policy st) (swId :: (switches st)));
+    _ <- config_commands (policy st) swId;
+    ret tt.
+
+  Definition body :=
+    evt <- recv;
+    match evt with
+      | SwitchDisconnected swId => handle_switch_disconnected swId
+      | SwitchConnected swId => handle_switch_connected swId
+      | SwitchMessage swId xid msg => ret tt
+    end.
+
+  Definition main := forever body.
+
+End Make.
